state.v
@@ -1,7 +1,6 @@
 Require Export FORYU.list_functions.
 Require Export FORYU.program.
 
-
 Module VariableAssignment(D: DIALECT).
 
   Module YULVariableMapD := YULVariableMap(D).
@@ -58,6 +57,88 @@ Module VariableAssignment(D: DIALECT).
     end.
 
 End VariableAssignment.
+
+(*
+
+Module VariableAssignment(D: DIALECT).
+
+  Module YULVariableMapD := YULVariableMap(D).
+  Module SimpleExprD := SimpleExpr(D).
+
+  (* Assignment from YUL variables to dialect values *)
+  Record t : Type := {
+      dom : VarSet.t;
+      f : YULVariable.t -> D.value_t
+    }.
+
+  (* Variables not initialized return the default value of the dialect *)
+
+  Definition empty : t := {| dom := VarSet.empty; f:= fun _ => D.default_value |}.
+  
+  Definition assign (assignment : t) (var : YULVariable.t) (value : D.value_t) : t :=
+    {|
+      dom := VarSet.add var (dom assignment);
+      f := fun v => if YULVariable.eqb v var then value else (f assignment) v
+    |}.
+
+  Definition get (assignment : t) (var : YULVariable.t) : D.value_t :=
+    (f assignment) var.
+ 
+  (* This get recieves a list of simple expressions *)
+  Definition get_se (assignment : t) (e : SimpleExprD.t) : D.value_t :=
+    match e with
+    | inl var => get assignment var
+    | inr val => val
+    end.
+
+  (* Returns a list of values for the given variables, if all variables are assigned. *)
+  (* If any variable is not assigned, returns None. *)
+  Definition get_all (assignments : t) (vars : list YULVariable.t) : list D.value_t :=
+    List.map (fun v => get assignments v) vars.
+
+  Definition get_all_se (assignments : t) (es : list SimpleExprD.t) : list D.value_t :=
+    List.map (fun e => get_se assignments e) es.
+
+  (* Takes a list of variables and a list of values and updates the assignment. If the list have 
+     different lengths, returns None  *)
+  Fixpoint assign_all (assignments : t) (vars : list YULVariable.t) (vals : list D.value_t) : option t :=
+    match vars, vals with
+    | nil, nil => Some assignments
+    | nil, _ :: _ => None
+    | _ :: _, nil => None
+    | var :: rvars, val :: rvals =>
+        match assign_all assignments rvars rvals with
+        | Some new_assignments => Some (assign new_assignments var val)
+        | None => None
+        end
+    end.
+
+  (* Applies a list of renamings to the assignments. Each renaming is a pair (dest, origin) where 
+     dest is the variable that will take the value of origin. *)
+  Fixpoint apply_renamings (assignments : t) (renamings : YULVariableMapD.t) : t :=
+    match renamings with
+    | nil => assignments
+    | (dest, origin) :: rest =>
+        apply_renamings (assign assignments dest (get_se assignments origin)) rest
+    end.
+
+
+  Definition Equal (a1 a2 : t) : Prop :=
+  (* 2. The functions are equal on all elements *in the domain* *)
+    (forall v, VarSet.In v (VarSet.union (dom a1) (dom a2)) -> (f a1) v = (f a2) v).
+
+        
+  Definition MyMap_eq_dec (a1 a2 : t) : {Equal a1 a2} + {~Equal a1 a2}.
+
+    destruct
+      (
+        let l1 := (map (fun var => (f a1) var) (VarSet.elements (VarSet.union (dom a1) (dom a2)))) in
+        let l2 := (map (fun var => (f a2) var) (VarSet.elements (VarSet.union (dom a1) (dom a2)))) in
+        list_eq_dec D.eq_dec l1 l2) as [H_l1_eq_l2 | H_l1_neq_l2].
+    - Search VarSet.elements.
+
+End VariableAssignment.
+*)
 
 
 Module StackFrame(D: DIALECT).
